Simplification of 'gencoqdec.ml'
git-svn-id: https://scm.gforge.inria.fr/anonscm/svn/simsoc-cert@1060 ce709078-17db-4df8-89f4-d3e5bb8270d9

pseudocode/dec.ml
@@ -87,6 +87,7 @@ sig
   val prefix_coq_main : string
   val display_cond : bool
   val decode_body : string list
+  val sort_inst : (Lightheadertype.lightheader * 'a) list -> (Lightheadertype.lightheader * 'a) list
 end
 
 module Arm : DEC =
@@ -112,11 +113,25 @@ struct
   let display_cond = true  
   let decode_body =
     [ "(w : word) : decoder_result inst :="
-    ; "  match w32_of_word w with"
-    ; "    | word32 1 1 1 1 _ _ _ _ _ _ _ _ _ _ _ _ _ _ _ _ _ _ _ _ _ _ _ _ _ _ _ _ =>"
-    ; "      decode_unconditional w"
+    ; "  match w32_first4bits_of_word w with"
+    ; "    | word4 1 1 1 1 => decode_unconditional w"
     ; "    | _ => decode_conditional w"
     ; "  end." ]
+
+  (* Numbers in pattern refers to instruction number, i.e.,
+   * the subsection in which the instruction is defined *)
+  let order_inst p =
+    match num p with
+      | 45|8|59|67|16|90 -> -6 (* instruction without condition *)
+      | 84|85|86|87|88|89|129|113|114|115|146|147|148 -> -1 (* instructions without accumulator *)
+      | 9|10|11|13|39|40 -> 1 (* v5 instructions with SBO or SBZ can hide other v6 instructions *)
+      | 25|105|31|101 -> 2 (* loadstore instructions with a 'T' *)
+      | 28|102|104|30|26|29 -> 3
+      | 38 -> 4
+      | 19|20|21|22|96|97|98|35|106|116|117|99|100|23|24|41
+      | 42|65|18|60|61|2|3|4|6|14|15 -> 5 (* other instuctions with a mode*)
+      | _ -> 0;;
+  let sort_inst l = List.sort (fun a b -> order_inst a - order_inst b) l
 end
 
 module Sh4 : DEC = 
@@ -135,4 +150,5 @@ struct
   let prefix_coq_main = "Sh4"
   let display_cond = false
   let decode_body = [ ":= decode_unconditional." ]
+  let sort_inst x = x
 end
